Grandpa/src/DataTypes/Dictionary.v
@@ -70,6 +70,53 @@ Proof.
         apply H2.
 Qed.
 
+Lemma add_aux_step_if_neq (k1 k2:K) (v1 v2:V) l 
+  (k1_neq_k2: k1 =? k2 =false)
+  : 
+  add_aux (k1,v1) ((k2,v2)::l) = (k2,v2)::add_aux (k1,v1) l.
+Proof.
+  simpl.
+  rewrite k1_neq_k2.
+  auto.
+Qed.
+
+Lemma add_aux_neq_at_begining (k1 k2:K) (v1 v2:V) l1 l2
+  (H: forall k', List.In k' (map fst l1) -> k1 =? k' = false)
+  : 
+  add_aux (k1,v1) (l1++l2) = l1++add_aux (k1,v1) l2.
+Proof.
+  induction l1.
+  - auto.
+  - enough (k1 =? fst a = false) as H2.
+    + simpl.
+      destruct a as [k3 v3].
+      simpl in H2.
+      rewrite H2.
+      rewrite IHl1.
+      ++ auto.
+      ++ simpl.
+         intros k4 H3.
+         apply H.
+         simpl.
+         right.
+         auto.
+    + apply H.
+      simpl.
+      left.
+      auto.
+Qed.
+
+Lemma add_aux_modifies_first_match (k1 k2:K) (v v':V) (l1 l2:list (K*V))
+  (eqb_k1_k2: k1 =? k2 = true)
+  (H: forall k', List.In k' (map fst l1) -> k1 =? k' = false)
+  : add_aux (k1,v) (l1++ (k2,v')::l2) = l1 ++ (k1,v)::l2.
+Proof.
+  rewrite (add_aux_neq_at_begining k1 k2 v v' l1 ((k2,v')::l2)).
+  - simpl.
+    rewrite eqb_k1_k2.
+    auto.
+  - auto.
+Qed.
 
 Definition add (k:K) (v:V) (dict:Dictionary K V): Dictionary K V
  := DictionaryC (add_aux (k,v) (to_list dict)).
@@ -154,7 +201,7 @@ Lemma lookup_add_result d :
   forall k1 k2 v, 
     let result := lookup k1 (add k2 v d) 
     in
-      (k1 =? k2 = true /\ result = Some v) \/ (result = lookup k1 d).
+      (k1 =? k2 = true /\ result = Some v) \/ ((k1 =? k2 = false) /\ (result = lookup k1 d)).
 Proof.
   intros k1 k2.
   destruct (k1 =? k2) eqn:k_eqb.
@@ -281,6 +328,7 @@ Proof.
   - simpl.
     auto using WellFormedAdd.
 Qed.
+
 
 Lemma wellformed_means_unique_elements d (wf:WellFormedDict d) 
   : forall k, 
