Grandpa/src/Protocol/FinalizedBlock.v
@@ -3,6 +3,7 @@ Require Import Votes.
 Require Import VoterState.
 Require Import Time.
 Require Import RoundNumber.
+Require Import OpaqueRound.
 
 
 (** *FinalizedBlock
@@ -21,6 +22,23 @@ Record FinalizedBlock := FinalizedBlockC {
   ;precommit_votes:Votes voters
   }.
 
+
+Definition make_with_round
+  (t:Time)
+  (voter:Voter) 
+  (b:AnyBlock)
+  (opaque:OpaqueRoundState)
+  : FinalizedBlock
+  := {|
+  block := b
+  ;time:=t
+  ;round_number:= OpaqueRound.get_round_number opaque
+  ;submitter_voter:=voter
+  ;voters:=OpaqueRound.get_precommit_voters opaque
+  ;precommit_votes:= OpaqueRound.get_all_precommit_votes opaque
+  |}.
+
+   
 (* TODO: 
    Maybe add make_with_round : Vote -> AnyBlock -> Round -> FinalizedBlock.
  *)
